updated utils to use ordmap over map

Fstar/fun/Implmenetations/Utils.fst
@@ -1,24 +1,23 @@
 module Utils
 
 // maybe change to generating OCaml maps!
-module Map = FStar.Map
+module Map = FStar.OrdMap
+module Set = FStar.OrdSet
 
 type addr = int
 
 unopteq type heap (a : Type) : Type = {
   size    : int;
   free    : l : (list int){Cons? l};
-  maps_to : Map.t int (option a)
+  maps_to : Map.ordmap int a (<=)
 }
 
 val h_initial (#a : Type) : (heap a)
 let h_initial #a = {
   size = 0;
   free = [1];
-  maps_to = Map.const None
+  maps_to = Map.empty
 }
-
-let test = Map.contains ((h_initial #int).maps_to) 2
 
 val h_alloc (#a : Type) : heap a -> a -> heap a * int
 let h_alloc #a {size; free; maps_to} v =
@@ -26,21 +25,36 @@ let h_alloc #a {size; free; maps_to} v =
   | [x] -> ({
     size    = size + 1;
     free    = [x + 1];
-    maps_to = Map.upd maps_to x (Some v)
+    maps_to = Map.update x v maps_to
     }, x)
   | x :: xs -> ({
     size    = size + 1;
     free    = xs;
-    maps_to = Map.upd maps_to x (Some v)
+    maps_to = Map.update x v maps_to
   }, x)
 
 val h_update (#a : Type) : heap a -> int -> a -> heap a
 let h_update #a heap key val' =
-  {heap with maps_to = Map.upd heap.maps_to key (Some val')}
+  {heap with maps_to = Map.update key val'  heap.maps_to}
 
 val h_free (#a : Type) : heap a -> int -> heap a
 let h_free #a {size; free; maps_to} key = {
   size    = size - 1;
   free    = key :: free;
-  maps_to = Map.upd maps_to key None
+  maps_to = Map.remove key maps_to
 }
+
+// For some reason as_list is private, but we can make it with fold
+private val set_as_list (#a:eqtype) (#acc:Type) (#f:Set.cmp a) : Set.ordset a f -> list a
+private let set_as_list #_ #_ #_ s =
+  Set.fold (fun acc x -> x :: acc) [] s
+
+val h_addresses (#a : Type) : heap a -> list int
+let h_addresses #a {size; free; maps_to} =
+   set_as_list #int #int (Map.dom maps_to)
+
+val h_lookup (#a : Type) : heap a -> int -> Prims.Tot (option a)
+let h_lookup #_ {maps_to} val' = Map.select val' maps_to
+
+val h_size (#a : Type) : heap a -> int
+let h_size #a = Mkheap?.size
